\section{Birth and Death Process}

\begin{definition}
Suppose that there are $ n $ people in the system, then the time $ B_{n} $ for a new member to join is exponential distribution with parameter $ \beta_{n} $, and the time $ D_{n} $ for a member to leave is exponential distribution with parameter $ \delta_{n} $. Such a system is called a \defterm{birth and death process}, and the parameters $ \{ \beta_{n} \}_{n \ge 0} $ and $ \{ \delta_{n} \}_{n \ge 0} $ are called \defterm{birth rate} and \defterm{death rate}, respectively.

Thus, the birth and death process is a continuous-time Markov chain with states $ \mathcal{S} = \{ 0, 1, \cdots \} $ for which transitions from state $ n $ may go only to either state $ n - 1 $ or $ n + 1 $, and
\begin{eqnarray*}
\forall(i \ge 2). \mathbb{P}[n, n \pm i] & = & 0, \\
\forall(n \le 1). \mathbb{P}[n, n - 1]
    & = & P(B_{n} > D_{n}) \\
    & = & \int_{0}^{\infty} P(B_{n} > t) \cdot P(D_{n} = t) \mathrm{d}t \\
    & = & \int_{0}^{\infty} e^{-\beta_{n}t} \cdot \delta_{n} \cdot e^{\delta_{n}t} \mathrm{d}t \\
    & = & \delta_{n} \int_{0}^{\infty} e^{-(\beta_{n} + \delta_{n})t} \mathrm{d}t \\
    & = & \frac{\delta_{n}}{\beta_{n} + \delta_{n}}, \\
\mathbb{P}[n, n + 1] & = & \frac{\beta_{n}}{\beta_{n} + \delta_{n}}.
\end{eqnarray*}
\end{definition}

\begin{example}
Poisson process with rate $ \lambda $: $ \beta_{n} = n $, $ \delta_{n} = 0 $.
\end{example}

\begin{example}
Yule process: birth process with linear birth. $ \beta_{n} = \lambda \cdot n $, $ \delta_{n} = 0 $.
\end{example}

\begin{example}
There are $ s $ servers. Jobs arrive at Poisson process with rate $ \lambda $, and the processing time is exponential with parameter $ \mu $. If all $ s $ servers are busy, there is a queue keeping the waiting jobs.

Let $ X(t) $ be the number of jobs in the system (including those in queue) at time $ t $, then $ \mathbb{X} $ is a birth and death process with $ \beta_{n} = \lambda $ and $ \delta_{n} = \mu \cdot \min \{n, s\} $.
\end{example}

\begin{question}
Linear growth model with immigration. $ \beta_{n} = \beta \cdot n + \delta $, $ \delta_{n} = \delta \cdot n $. $ E[X(t)] $ = ?
\begin{alignat*}{3}
  & \forall (n \ge 0). P(X(t + h) = n + 1 \mid X(t) = n)
    & \quad=\quad & (\beta \cdot n + \theta) \cdot h + o(h), \\
  & \forall (n \ge 1). P(X(t + h) = n - 1 \mid X(t) = n)
    & \quad=\quad & \delta \cdot n \cdot h + o(h), \\
  & \forall (n \ge 0). P(X(t + h) = n \mid X(t) = n)
    & \quad=\quad & 1 - (\beta \cdot n + \delta \cdot n + \theta) \cdot h + o(h), \\
  & \text{all others are $ o(h) $.} \\
\Rightarrow\quad
  & P(X(t + h) = X(t) + 1)
    & \quad=\quad & (\beta \cdot X(t) + \theta) \cdot h + o(h), \\
  & P(X(t + h) = X(t) - 1)
    & \quad=\quad & \delta \cdot X(t) \cdot h + o(h), \\
  & P(X(t + h) = X(t))
    & \quad=\quad & 1 - (\beta \cdot X(t) + \delta \cdot X(t) + \theta) \cdot h + o(h), \\
  & P(|X(t + h) = X(t)| > 1)
    & \quad=\quad & o(h). \\
\Rightarrow\quad
  & E[X(t + h) \mid X(t)]
    & \quad=\quad & (X(t) + 1) \cdot [(\beta \cdot X(t) + \theta) \cdot h + o(h)] \\
  & & & + (X(t) + 1) \cdot (\delta \cdot X(t) \cdot h + o(h)) \\
  & & & + X(t) \cdot [1 - (\beta \cdot X(t) + \delta \cdot X(t) + \theta) \cdot h + o(h)] \\
  & & \quad=\quad & X(t) + [(\beta - \delta) \cdot X(t) + \theta] \cdot h + o(h). \\
\Rightarrow\quad
  & E[X(t + h)]
    & \quad=\quad & [1 + (\beta - \delta) \cdot h] \cdot E[X(t)] + \theta \cdot h + o(h). \\
\Rightarrow\quad
  & \frac{E[X(t + h)] - E[X(t)]}{h}
    & \quad=\quad & (\beta - \delta) \cdot E[X(t)] + \theta + \frac{o(h)}{h}. \\
\Rightarrow\quad
  & \frac{\mathrm{d}}{\mathrm{d}t} E[X(t)]
    & \quad=\quad & (\beta - \delta) \cdot E[X(t)] + \theta. \\
\end{alignat*}

Thus,
\begin{itemize}
\item If $ \beta = \delta $, then $ \frac{\mathrm{d}}{\mathrm{d}t} E[X(t)] = \theta $.

\item If $ \beta \neq \delta $, then
\[ E[X(t)] = X(0) \cdot e^{(\beta - \delta)t} + \frac{\theta}{(\beta - \delta)} \cdot (e^{(\beta - \delta)t} - 1). \]
\end{itemize}

\begin{comment}
If $ \beta < \delta $,
\[ \lim_{t \to \infty} E[X(t)] = \frac{\theta}{\delta - \beta} > 0. \]
\end{comment}
\end{question}

\begin{definition}
The \defterm{increment time} $ T_{i} $ for state $ i $ in a birth and death process $ \mathbb{X} $ is the time from state $ i $ to reach state $ i + 1 $. Given $ X(0) = i $,
\[ T_{i} = \min_{t} \{ t \mid X(t) = i + 1 \}. \]
\end{definition}

\begin{question}
$ E[T_{i}] $ = ?

\begin{itemize}
\item $ i = 0 $: $ E[T_{0}] = 1 / \beta_{0} $. \\
  因為 $ T_{0} $ 一定是 exponential distribution with parameter $ \beta_{0} $。

\item $ i > 0 $: Let
\[ I_{i} = \begin{cases}
1 & \text{if the first transition is an increment (birth),} \\
0 & \text{otherwise.}
\end{cases} \]
and hence
\begin{eqnarray*}
E[T_{i} \mid I_{i} = 1] & = & \frac{1}{\beta_{i} + \delta_{i}}, \\
E[T_{i} \mid I_{i} = 0] & = & \underbrace{\frac{1}{\beta_{i} + \delta_{i}}}_{i \to i - 1} + \underbrace{E[T_{i - 1}]}_{i - 1 \to i} + \underbrace{E[T_{i}]}_{i \to i + 1}.
\end{eqnarray*}

Therefore,
\begin{alignat*}{3}
  & E[T_{i} \mid I_{i}]
    & \quad=\quad & \frac{1}{\beta_{i} + \delta_{i}} + (1 - I_{i}) \cdot (E[T_{i - 1}] + E[T_{i}]) \\
\Rightarrow\quad
  & E[T_{i}]
    & \quad=\quad & E[E[T_{i} \mid I_{i}]] \\
  & & \quad=\quad & \frac{1}{\beta_{i} + \delta_{i}} + (1 - E[I_{i}]) \cdot (E[T_{i - 1}] + E[T_{i}]) \\
  & & \quad=\quad & \frac{1}{\beta_{i} + \delta_{i}} + \left( 1 - \frac{\delta_{i}}{\beta_{i} + \delta_{i}} \right) \cdot (E[T_{i - 1}] + E[T_{i}]) \\
\Rightarrow\quad
  & E[T_{i}]
    & \quad=\quad & \frac{\delta_{i} \cdot E[T_{i - 1}]}{\beta_{i}}.
\end{alignat*}
\end{itemize}
\end{question}

\begin{example}
Constant-rate process: $ \beta_{n} = \beta $ and $ \delta_{n} = \delta $ for all $ n $.
\[ E[T_{i}] = \frac{1}{\beta_{0}} \cdot \sum_{j = 0}^{n} \left( \frac{\delta}{\beta} \right)^{i}. \]
\end{example}
