\section{Transition Probability Function}

\begin{definition}
For states $ i $ and $ j $, the \defterm{transition probability function} from $ i $ to $ j $ is
\[ p_{i, j}(t) = P(X(t) = j \mid X(0) = i). \]
\end{definition}

\begin{lemma}
If $ \mathbb{X} $ is a pure-birth process ($ \forall n \in \mathcal{S}. \delta_{n} = 0 $),
\[ p_{i, j}(t) = \begin{cases}
e^{-\beta_{i}t}               & \text{if } i = j, \\
Q_{i, j}(t) - Q_{i, j - 1}(t) & \text{if } i < j.
\end{cases} \]
where $ Q_{i, j}(t) = P(T_{i} + T_{i + 1} + \cdots + T_{j} > t) $, and $ T_{i} $ is the waiting time of state $ i $.
\begin{proof}
\begin{itemize}
\item If $ i = j $,
\begin{eqnarray*}
p_{i, i}(t)
  & = & P(T_{i} > t) \\
  & = & 1 - P(T_{i} \le t) \\
  & = & 1 - (1 - e^{-\beta_{i}t}) \\
  & = & e^{-\beta_{i}t}.
\end{eqnarray*}

\item If $ i < j $,
\begin{eqnarray*}
P(X(t) < j \mid X(0) = i)
  & = & P(T_{i} + T_{i + 1} + \cdots + T_{j - 1} > t) \\
  & = & Q_{i, j - 1}(t), \\
p_{i, j}(t)
  & = & P(X(t) = j \mid X(0) = i) \\
  & = & P(X(t) < j + 1 \mid X(0) = i) - P(X(t) < j \mid X(0) = i) \\
  & = & Q_{i, j}(t) - Q_{i, j - 1}(t).
\end{eqnarray*}
\end{itemize}
\end{proof}
\end{lemma}

\begin{example}
Yule process: $ \beta_{n} = n \cdot \beta $, $ \delta_{n} = 0 $.
\begin{eqnarray*}
Q_{i, j}(t) 
  & {\color{red}=} & \sum_{k = i}^{j} e^{\beta_{k}t} \cdot \prod_{r = i}^{j} \frac{\beta_{r}}{\beta_{r} - \beta_{k}} \\
  &   & \color{gray}{(\text{這裡有用到 $ T_{i}, T_{i + 1}, \cdots, T_{j - 1} $ 是參數「相異」指數分佈的性質})} \\
  & = & \sum_{k = i}^{j} e^{\beta_{k}t} \cdot \prod_{r = i}^{j} \frac{r}{r - k} \\
  & {\color{red}=} & e^{\beta_{j}t} \cdot \prod_{r = i}^{j} \frac{r}{r - j} + \sum_{k = i}^{j - 1} e^{\beta_{k}t} \cdot \prod_{r = i}^{j} \frac{j - 1}{(i - k)(i + 1 - k) \cdots (j - k)} \\
p_{1, j}(t)
  & {\color{red}=} & e^{\beta_{j}t} (1 - e^{\beta_{j}t})^{j - 1}.
\end{eqnarray*}
可知 $ p_{1, j}(t) $ 為 geometric distribution with parameter $ p = e^{-\beta t} $，且 $ p_{i, j}(t) $ 為 negative binomial distribution with param $ (i, p) $，因為 $ i $ 個 geometric 相加為 negative binomial。

That is,
\[ p_{i, j}(t) = {{j - 1}\choose{i - 1}} \cdot e^{-\beta_{i}t}(1 - e^{-\beta_{i}t})^{j - i}. \]
\end{example}

\begin{definition}
For states $ i $ and $ j $, the \defterm{instantaneous transition rate} is
\[ q_{i, j} = \begin{cases}
0                                   & \text{if } i = j, \\
\lambda_{i} \cdot \mathbb{P}[i, j]  & \text{if } i \neq j.
\end{cases} \]
\begin{comment}
$ \lambda_{i} $ 是離開 state $ i $ 的 Poisson rate；$ \lambda_{i} \cdot \mathbb{P}[i, j] $ 是離開 state $ i $ 、跑到 state $ j $ 的 Poisson rate。
\end{comment}
\begin{comment}
\begin{eqnarray*}
\lambda_{i}
  & = & \sum_{j \in \mathcal{S}} \lambda_{i} \cdot \mathbb{P}[i, j] \\
  & = & \sum_{j \in \mathcal{S}} q_{i, j}, \\
\mathbb{P}[i, j]
  & = & \frac{q_{i, j}}{\lambda_{i}} \\
  & = & \frac{q_{i, j}}{\sum_{j \in \mathcal{S}} q_{i, j}}.
\end{eqnarray*}
\end{comment}
\end{definition}

\subsection{Kolmogorov's Equations}

\begin{theorem}[backward equation] \label{thm:backward_eq}
For any $ \mathbb{X} $,
\[ p'_{i, j}(t) + \lambda_{i} \cdot p_{i, j}(t) = \sum_{k \in \mathcal{S}} q_{i, k} \cdot p_{k, j}(t). \]
\end{theorem}

\begin{theorem}[forward equation] \label{thm:forward_eq}
For almost any $ \mathbb{X} $,
\[ p'_{i, j}(t) + \lambda_{i} \cdot p_{i, j}(t) = \sum_{k \in \mathcal{S}} p_{i, k}(t) \cdot q_{k, j}. \]
\end{theorem}

\begin{example}
Pure-birth process: $ \mathbb{P}[i, i + 1] = 1, \delta_{n} = 0 $.

By \nameref{thm:backward_eq},
\begin{eqnarray*}
p'_{i, j}(t)
  & = & \lambda_{i} \cdot \mathbb{P}[i, i + 1] \cdot p_{i + 1, j}(t) - \lambda_{i} \cdot p_{i, j}(t) \\
  & = & \beta_{i} \cdot p_{i + 1, j}(t) - \beta_{i} \cdot p_{i, j}(t).
\end{eqnarray*}
\end{example}

\begin{example} \label{ex:backward_birth_and_death}
Birth and death process:
\begin{eqnarray*}
\mathbb{P}[i, i + 1] & = & \frac{\beta_{i}}{\beta_{i} + \delta_{i}} \\
\mathbb{P}[i, i - 1] & = & \frac{\delta_{i}}{\beta_{i} + \delta_{i}} \\
\mathbb{P}[i, i] & = & 1.
\end{eqnarray*}

By \nameref{thm:backward_eq}, if $ i = 0 $,
\[ p'_{0, j} = \beta_{0} \cdot p_{1, j}(t) - \beta_{0} \cdot p_{0, j}(t). \]
If $ i > 0 $,
\begin{eqnarray*}
p'_{i, j}
  & = & (\beta_{i} + \delta_{i}) \left( \frac{\beta_{i}}{\beta_{i} + \delta_{i}} \cdot p_{i + 1, j}(t) + \frac{\delta_{i}}{\beta_{i} + \delta_{i}} \cdot p_{i - 1, j}(t) - p_{i, j}(t) \right) \\
  & = & \beta_{i} \cdot p_{i + 1, j}(t) + \delta_{i} \cdot p_{i - 1, j}(t) - (\beta_{i} + \delta_{i}) \cdot p_{i, j}(t).
\end{eqnarray*}
\end{example}

\begin{question}
$ \mathbb{X} $ is a birth and death process with 2 states, and $ \beta_{0} = \beta, \delta_{1} = \delta, \beta_{1} = \delta_{0} = 0 $. $ p_{0, 0} $ = ? $ p_{1, 0} $ = ?

According to \autoref{ex:backward_birth_and_death},
\begin{eqnarray*}
p'_{0, 0}(t) & = & \beta (p_{1, 0}(t) - p_{0, 0}(t)), \\
p'_{1, 0}(t) & = & \delta (p_{0, 0}(t) - p_{1, 0}(t)).
\end{eqnarray*}

Thus,
\begin{eqnarray*}
p_{0, 0}(t) & = & \frac{\beta}{\beta + \delta} \cdot e^{-(\beta + \delta)t} + \frac{\delta}{\beta + \delta}, \\
p_{1, 0}(t) & = & \frac{\delta}{\beta + \delta} - \frac{\delta}{\beta + \delta} \cdot e^{-(\beta + \delta)t}.
\end{eqnarray*}
\end{question}
