\section{Mean Time Spent in Transient States}

\begin{definition}
For any states $ i $ and $ j $,
\begin{itemize}
  \item let $ s_{ij} $ denote the \defterm{excepted number of time indices} $ t \ge 0 $ with $ X(t) = j $ given $ X(0) = i $,
  \item let $ f_{ij} $ be the probability $ P(\exists t \ge 1 . X(t) = j \mid X(0) = i) $.
\end{itemize}

\begin{comment}
只需考慮 $ i \to j $ 且 $ i, j $ 都是 transient 的情況。

\begin{itemize}
  \item $ i \not\to j \Rightarrow s_{ij} = 0 $.
  \item $ i \to j \wedge i \text{ is recurrent} \Rightarrow s_{ij} = \infty $. \\
    ($ i \to j \wedge i \text{ is recurrent} \Rightarrow j \to i \Rightarrow j $ is recurrent.)
  \item $ i \to j \wedge j \text{ is recurrent} \Rightarrow s_{ij} = \infty $. \\
    (有 $ > 0 $ 的機率會回到 $ j $，且之後會一直回到 $ j $。)
\end{itemize}
\end{comment}
\end{definition}

\begin{theorem}
Let $ \mathcal{T} $ consist of transient states of $ \mathbb{X} $, and $ \mathbb{P}_{\mathcal{T}} $ be the submatrix of $ \mathbb{P} $ induced by $ \mathcal{T} $. Then,
\begin{eqnarray*}
s_{ij} & = & (\mathbb{I} - \mathbb{P}_{\mathcal{T}})^{-1}[i, j], \\
f_{ij} & = & \frac{s_{ij} - \delta_{ij}}{s_{jj}},
\end{eqnarray*}
where
\[ \delta_{ij} = \begin{cases}
  1 & \text{if } i = j, \\
  0 & \text{otherwise}.
\end{cases} \]

\begin{proof}[proof ($ s_{ij} $)]
If $ k $ is recurrent and hence $ k \in \mathcal{S} - \mathcal{T} $, then $ k \not\to j $ (since $ j $ is transient). Thus, $ s_{kj} = 0 $ and
\begin{eqnarray*}
s_{ij}
  & = & \delta_{ij} + \sum_{k \in \mathcal{S}} \mathbb{P}[i, k] \cdot s_{kj} \\
  & = & \delta_{ij} + \sum_{k \in \mathcal{T}} \mathbb{P}[i, k] \cdot s_{kj}. \\
\end{eqnarray*}

Let $ \mathbb{S}[i, j] = s_{ij} $,
\begin{eqnarray*}
  & & \mathbb{I}\,\mathbb{S} = \mathbb{S} = \mathbb{I} + \mathbb{P}_{\mathcal{T}} \mathbb{S} \\
  & \Rightarrow & (\mathbb{I} - \mathbb{P}_{\mathcal{T}})\mathbb{S} = \mathbb{I} \\
  & \Rightarrow & \mathbb{S} = (\mathbb{I} - \mathbb{P}_{\mathcal{T}})^{-1}.
\end{eqnarray*}
\end{proof}

\begin{proof}[proof ($ f_{ij} $)]
Conditioned on whether there exists an index $ t $ with $ X(t) = j $ (and $ j \not\in \{ X(1), \cdots, X(t - 1) \} $),
$ s_{ij} = \sum_{t = 1}^{\infty} P(X(t) = j \mid X(0) = i) \cdot t $
\begin{eqnarray*}
  & & s_{ij} = \underbrace{\delta_{ij}}_{t = 0}  + \underbrace{s_{jj} \cdot f_{ij}}_{t \ge 1} \\
  & \Rightarrow & f_{ij} = \frac{s_{ij} - \delta_{ij}}{s_{jj}}.
\end{eqnarray*}
\end{proof}
\end{theorem}

\begin{example}
\begin{figure}[htp]
\centering
\begin{tikzpicture}[node distance=6em]
  \node[state] (X0) {$ 0 $};
  \foreach \x in {1,...,5}{
    \pgfmathtruncatemacro{\y}{\x - 1}
    \node[state] (X\x) [right of=X\y] {$ \x $};
  }

  \path (X0) edge [loop left] node {1} (X0)
        (X1) edge [bend right=0] node [swap] {0.5} (X0)
        (X4) edge [bend right=0] node {0.5} (X5)
        (X5) edge [loop right] node {1} (X5);
  \foreach \x in {2,...,4}{
    \pgfmathtruncatemacro{\y}{\x - 1}
    \path[<->] (X\y) edge [bend right=0] node {$ 0.5 $} (X\x);
  }
\end{tikzpicture}
\end{figure}

\begin{multicols}{2}
\[ \mathbb{P} = \bordermatrix{
    & 0 & 1 & 2 & 3 & 4 & 5 \cr
  0 & 1 & 0 & 0 & 0 & 0 & 0 \cr
  1 & \frac{1}{2} & 0 & \frac{1}{2} & 0 & 0 & 0 \cr
  2 & 0 & \frac{1}{2} & 0 & \frac{1}{2} & 0 & 0 \cr
  3 & 0 & 0 & \frac{1}{2} & 0 & \frac{1}{2} & 0 \cr
  4 & 0 & 0 & 0 & \frac{1}{2} & 0 & \frac{1}{2} \cr
  5 & 0 & 0 & 0 & 0 & 0 & 1 \cr
} \]

\null \vfill
\null \vfill
\begin{eqnarray*}
\mathbb{S} = (\mathbb{I} - \mathbb{P}_{\mathcal{T}})^{-1} & = & \begin{pmatrix}
  1.6 & 1.2 & 0.8 & 0.4 \\
  1.2 & 2.4 & 1.6 & 0.8 \\
  0.8 & 1.6 & 2.4 & 1.2 \\
  0.4 & 0.8 & 1.2 & 1.6 \\
\end{pmatrix} \\
\mathbb{F} & = & \begin{pmatrix}
  \frac{3}{8} & \frac{1}{2}     & \frac{1}{3}     & \frac{1}{4} \\
  \frac{3}{4} & \frac{7}{12}  & \frac{19}{30}   & \frac{1}{2} \\
  \frac{1}{2} & \frac{19}{30}   & \frac{7}{12}  & \frac{3}{4} \\
  \frac{1}{4} & \frac{1}{3}     & \frac{1}{2}     & \frac{3}{8}
\end{pmatrix}
\end{eqnarray*}
\end{multicols}
\end{example}